@prefix owl: <http://www.w3.org/2002/07/owl#> .
@prefix rdfs: <http://www.w3.org/2000/01/rdf-schema#> .
@prefix ewe: <http://gsi.dit.upm.es/ontologies/ewe/ns/> .
@prefix rdf: <http://www.w3.org/1999/02/22-rdf-syntax-ns#> .
@prefix ex: <http://example.org/ex#> .
@prefix dogont: <http://elite.polito.it/ontologies/dogont.owl#> .
@prefix foaf: <http://xmlns.com/foaf/0.1/> .
@prefix ewe-device: <http://gsi.dit.upm.es/ontologies/ewe-device/ns/> .
@prefix xsd: <http://www.w3.org/2001/XMLSchema#> .
@base  <http://gsi.dit.upm.es/ontologies/ewe/ns/> .


###################################
# Channel definition
###################################
ewe:PlantSensor a owl:Class ;    
    rdfs:label "plant sensor" ;
    rdfs:comment "This channel represents a plant sensor." ;
    foaf:logo "fa fa-tree" ;
    ewe:generatesEvent ewe:PlantMoistureLowerThan ;
    ewe:generatesEvent ewe:PlantMoistureGreaterThan ;
    ewe:generatesEvent ewe:PlantLightLowerThan ;
    ewe:generatesEvent ewe:PlantLightGreaterThan ;
    ewe:generatesEvent ewe:PlantTemperatureLowerThan ;
    ewe:generatesEvent ewe:PlantTemperatureGreaterThan ;
    ewe:generatesEvent ewe:PlantConductivityLowerThan ;
    ewe:generatesEvent ewe:PlantConductivityGreaterThan ;
    ewe:hasCategory ewe-device:Device ;
    rdfs:subClassOf ewe:Channel .


###################################
# Events definition
###################################

ewe:PlantMoistureLowerThan a owl:Class ;
    rdfs:label "Plant moisture detected lower than the specified parameter" ;
    rdfs:comment "This event will be triggered when the plant does not exceed the specified moisture." ;
    ewe:hasOutputParameter ewe:SensorID ;
    ewe:hasOutputParameter ewe:Moisture ;
    rdfs:subClassOf ewe:Event ;
    rdfs:domain ewe:plantSensor .

ewe:PlantMoistureGreaterThan a owl:Class ;
    rdfs:label "Plant moisture detected greater than the specified parameter" ;
    rdfs:comment "This event will be triggered when the plant exceeds the specified moisture." ;
    ewe:hasOutputParameter ewe:SensorID ;
    ewe:hasOutputParameter ewe:Moisture ;
    rdfs:subClassOf ewe:Event ;
    rdfs:domain ewe:plantSensor .

ewe:PlantLightLowerThan a owl:Class ;
    rdfs:label "Plant luminosity detected lower than the specified parameter" ;
    rdfs:comment "This event will be triggered when the plant does not exceed the specified luminosity." ;
    ewe:hasOutputParameter ewe:SensorID ;
    ewe:hasOutputParameter ewe:Light ;
    rdfs:subClassOf ewe:Event ;
    rdfs:domain ewe:plantSensor .

ewe:PlantLightGreaterThan a owl:Class ;
    rdfs:label "Plant luminosity detected greater than the specified parameter" ;
    rdfs:comment "This event will be triggered when the plant exceeds the specified luminosity." ;
    ewe:hasOutputParameter ewe:SensorID ;
    ewe:hasOutputParameter ewe:Light ;
    rdfs:subClassOf ewe:Event ;
    rdfs:domain ewe:plantSensor .

ewe:PlantTemperatureLowerThan a owl:Class ;
    rdfs:label "Plant temperature detected lower than the specified parameter" ;
    rdfs:comment "This event will be triggered when the plant does not exceed the specified temperature." ;
    ewe:hasOutputParameter ewe:SensorID ;
    ewe:hasOutputParameter ewe:Temperature ;
    rdfs:subClassOf ewe:Event ;
    rdfs:domain ewe:plantSensor .

ewe:PlantTemperatureGreaterThan a owl:Class ;
    rdfs:label "Plant temperature detected greater than the specified parameter" ;
    rdfs:comment "This event will be triggered when the plant exceeds the specified temperature." ;
    ewe:hasOutputParameter ewe:SensorID ;
    ewe:hasOutputParameter ewe:Temperature ;
    rdfs:subClassOf ewe:Event ;
    rdfs:domain ewe:plantSensor .

ewe:PlantConductivityLowerThan a owl:Class ;
    rdfs:label "Plant soil conductivity detected lower than the specified parameter" ;
    rdfs:comment "This event will be triggered when the plant does not exceed the specified soil conductivity." ;
    ewe:hasOutputParameter ewe:SensorID ;
    ewe:hasOutputParameter ewe:Conductivity ;
    rdfs:subClassOf ewe:Event ;
    rdfs:domain ewe:plantSensor .

ewe:PlantConductivityGreaterThan a owl:Class ;
    rdfs:label "Plant soil conductivity detected greater than the specified parameter" ;
    rdfs:comment "This event will be triggered when the plant exceeds the specified soil conductivity." ;
    ewe:hasOutputParameter ewe:SensorID ;
    ewe:hasOutputParameter ewe:Conductivity ;
    rdfs:subClassOf ewe:Event ;
    rdfs:domain ewe:plantSensor .
    
###################################
# Actions definition
###################################
# This channel has not actions


###################################
# Parameters definition
###################################

ewe:SensorID a owl:Class ;
    rdfs:label "Sensor ID" ;
    rdfs:comment "This parameter represents sensor ID." ;
    rdf:datatype xsd:string ;
    rdfs:subClassOf ewe:Parameter ;
    rdfs:domain ewe:plantSensor .

ewe:Moisture a owl:Class ;
    rdfs:label "Plant moisture measured" ;
    rdfs:comment "This parameter represents the moisture measured by the sensor." ;
    rdf:datatype xsd:math ;
    rdfs:subClassOf ewe:Parameter ;
    rdfs:domain ewe:plantSensor .

ewe:Light a owl:Class ;
    rdfs:label "Plant luminosity measured" ;
    rdfs:comment "This parameter represents the luminosity measured by the sensor." ;
    rdf:datatype xsd:math ;
    rdfs:subClassOf ewe:Parameter ;
    rdfs:domain ewe:plantSensor .

ewe:Temperature a owl:Class ;
    rdfs:label "Plant temperature measured" ;
    rdfs:comment "This parameter represents the temperature measured by the sensor." ;
    rdf:datatype xsd:math ;
    rdfs:subClassOf ewe:Parameter ;
    rdfs:domain ewe:plantSensor .

ewe:Conductivity a owl:Class ;
    rdfs:label "Plant soil conductivity measured" ;
    rdfs:comment "This parameter represents the soil conductivity measured by the sensor." ;
    rdf:datatype xsd:math ;
    rdfs:subClassOf ewe:Parameter ;
    rdfs:domain ewe:plantSensor .


###################################
# Example of instances
###################################

#ex:samsungtv rdf:type ewe-smarttv:SmartTv .

#ex:showimg1 rdf:type ewe-smarttv:DisplayImage ;
#    ewe:generatedBy ex:samsungtv ;
#    ewe:time "2016-01-19T15:10:00Z" .

# Generated facts 

#ex:labdoor1 rdf:type dogont:DoorActuator .