@prefix owl: <http://www.w3.org/2002/07/owl#> .
@prefix rdfs: <http://www.w3.org/2000/01/rdf-schema#> .
@prefix ewe: <http://gsi.dit.upm.es/ontologies/ewe/ns/> .
@prefix rdf: <http://www.w3.org/1999/02/22-rdf-syntax-ns#> .
@prefix ex: <http://example.org/ex#> .
@prefix dogont: <http://elite.polito.it/ontologies/dogont.owl#> .
@prefix foaf: <http://xmlns.com/foaf/0.1/> .
@prefix ewe-device: <http://gsi.dit.upm.es/ontologies/ewe-device/ns/> .
@prefix dbo: <http://dbpedia.org/ontology/> .
@prefix xsd: <http://www.w3.org/2001/XMLSchema#> .
@base  <http://gsi.dit.upm.es/ontologies/ewe/ns/> .


###################################
# Channel definition
###################################
ewe:PresenceSensor a owl:Class ;    
    rdfs:label "Presence sensor" ;
    rdfs:comment "This channel represents a presence sensor." ;
    foaf:logo "fa fa-street-view" ;
    dbo:colour dbo:Purple ;
    ewe:generatesEvent ewe:PresenceDetectedAtDistanceLessThan ;
    ewe:generatesEvent ewe:PresenceDetectedAtDistanceGreaterThan ;
    ewe:generatesEvent ewe:PresenceNotDetectedInTime ;
    ewe:hasCategory ewe-device:Device ;
    rdfs:subClassOf ewe:Channel .


###################################
# Events definition
###################################
ewe:PresenceDetectedAtDistanceLessThan a owl:Class ;
    rdfs:label "Presence detected at distance less than the specified parameter" ;
    rdfs:comment "This event will be triggered when presence sensor detects a user closer than the specified distance." ;
    ewe:hasInputParameter ewe:PresenceSensorID ;
    ewe:hasOutputParameter ewe:PresenceDistance ;
    rdfs:subClassOf ewe:Event ;
    rdfs:domain ewe:PresenceSensor .

ewe:PresenceNotDetectedInTime a owl:Class ;
    rdfs:label "Presence not detected during the specified parameter" ;
    rdfs:comment "This event will be triggered when presence sensor is not detected a user during an specified time." ;
    ewe:hasInputParameter ewe:PresenceSensorID ;
    ewe:hasOutputParameter ewe:PresenceTime ;
    rdfs:subClassOf ewe:Event ;
    rdfs:domain ewe:PresenceSensor .

ewe:PresenceDetectedAtDistanceGreaterThan a owl:Class ;
    rdfs:label "Presence detected at distance greater than the specified parameter" ;
    rdfs:comment "This event will be triggered when presence sensor detects a user far than the specified distance." ;
    ewe:hasInputParameter ewe:PresenceSensorID ;
    ewe:hasOutputParameter ewe:PresenceDistance ;
    rdfs:subClassOf ewe:Event ;
    rdfs:domain ewe:PresenceSensor .

    
###################################
# Actions definition
###################################
# This channel has not actions


###################################
# Parameters definition
###################################

ewe:PresenceSensorID a owl:Class ;
    rdfs:label "Presence Sensor ID" ;
    rdfs:comment "This parameter represents the presence sensor ID." ;
    rdf:datatype xsd:string ;
    rdfs:subClassOf ewe:Parameter ;
    rdfs:domain ewe:PresenceSensor .

ewe:PresenceDistance a owl:Class ;
    rdfs:label "Distance in meters" ;
    rdfs:comment "This parameter represents the distance measured by the presence sensor." ;
    rdf:datatype xsd:math ;
    rdfs:subClassOf ewe:Parameter ;
    rdfs:domain ewe:PresenceSensor .

ewe:PresenceTime a owl:Class ;
    rdfs:label "Time in seconds" ;
    rdfs:comment "This parameter represents the period of time measured by the presence sensor." ;
    rdf:datatype xsd:math ;
    rdfs:subClassOf ewe:Parameter ;
    rdfs:domain ewe:PresenceSensor .

###################################
# Example of instances
###################################

#ex:samsungtv rdf:type ewe-smarttv:SmartTv .

#ex:showimg1 rdf:type ewe-smarttv:DisplayImage ;
#    ewe:generatedBy ex:samsungtv ;
#    ewe:time "2016-01-19T15:10:00Z" .

# Generated facts 

#ex:labdoor1 rdf:type dogont:DoorActuator .